Sparsity...

LogicalRefinement/Stlc/Interp.lean
@@ -42,69 +42,12 @@ def Context.stlc: Context -> Stlc.Context
 | (Hyp.mk A (HypKind.val type))::Hs => A.stlc_ty::(stlc Hs)
 | H::Hs => stlc Hs
 
-def Sparsity := List Bool
-
 def Hyp.sparsity: Hyp -> Bool
 | Hyp.mk A k => k == HypKind.val type
 
 def Context.sparsity: Context -> Sparsity
 | [] => []
 | H::Hs => H.sparsity::(sparsity Hs)
-
-@[simp]
-def Sparsity.dep: Sparsity -> Nat -> Bool
-| [], n => true
-| b::Hs, 0 => b
-| b::Hs, Nat.succ n => dep Hs n
-
-theorem Sparsity.dep_get? {Γ: Sparsity} {n b}
-  : Γ.get? n = some b -> Γ.dep n = b
-  := by {
-    revert n;
-    induction Γ with
-    | nil => intro n H; cases H
-    | cons H Γ I =>
-      intro n Hn;
-      cases n with
-      | zero => simp [List.get?] at Hn; simp [Hn]
-      | succ n => simp only [dep, I Hn]
-  }
-
-def Sparsity.wknth: Sparsity -> Nat -> Bool -> Sparsity
-| H::Γ, Nat.succ n, b => H::(wknth Γ n b)
-| [], Nat.succ n, b => true::(wknth [] n b)
-| Γ, 0, b => b::Γ
-
-@[simp]
-def Sparsity.ix: Sparsity -> Nat -> Nat
-| true::Hs, Nat.succ n => (ix Hs n) + 1
-| false::Hs, Nat.succ n => ix Hs n
-| _, n => n
-
-@[simp]
-def Sparsity.ix_inv: Sparsity -> Nat -> Nat
-| true::Hs, Nat.succ n => (ix_inv Hs n) + 1
-| false::Hs, n => (ix_inv Hs n) + 1
-| _, n => n
-
-def Sparsity.ix_inv_valid (Γ: Sparsity) {n: Nat}:
-  Γ.dep n = true -> Γ.ix_inv (Γ.ix n) = n
-  := by {
-    revert n;
-    induction Γ with
-    | nil => intro n H; rfl
-    | cons H Γ I =>
-      intro n;
-      cases n with
-      | zero => 
-        intro Hn;
-        cases H with
-        | true => rfl
-        | false => simp [List.get?] at Hn
-      | succ n =>
-        intro Hn;
-        cases H <;> simp [ix, ix_inv, I Hn] 
-  }
 
 def Context.stlc_ix (Γ: Context): Nat -> Nat := Γ.sparsity.ix
 
