LogicalRefinement/Stlc/Sparsity.lean
@@ -1,0 +1,57 @@
+def Sparsity := List Bool
+
+
+@[simp]
+def Sparsity.dep: Sparsity -> Nat -> Bool
+| [], n => true
+| b::Hs, 0 => b
+| b::Hs, Nat.succ n => dep Hs n
+
+theorem Sparsity.dep_get? {Γ: Sparsity} {n b}
+  : Γ.get? n = some b -> Γ.dep n = b
+  := by {
+    revert n;
+    induction Γ with
+    | nil => intro n H; cases H
+    | cons H Γ I =>
+      intro n Hn;
+      cases n with
+      | zero => simp [List.get?] at Hn; simp [Hn]
+      | succ n => simp only [dep, I Hn]
+  }
+
+def Sparsity.wknth: Sparsity -> Nat -> Bool -> Sparsity
+| H::Γ, Nat.succ n, b => H::(wknth Γ n b)
+| [], Nat.succ n, b => true::(wknth [] n b)
+| Γ, 0, b => b::Γ
+
+@[simp]
+def Sparsity.ix: Sparsity -> Nat -> Nat
+| true::Hs, Nat.succ n => (ix Hs n) + 1
+| false::Hs, Nat.succ n => ix Hs n
+| _, n => n
+
+@[simp]
+def Sparsity.ix_inv: Sparsity -> Nat -> Nat
+| true::Hs, Nat.succ n => (ix_inv Hs n) + 1
+| false::Hs, n => (ix_inv Hs n) + 1
+| _, n => n
+
+def Sparsity.ix_inv_valid (Γ: Sparsity) {n: Nat}:
+  Γ.dep n = true -> Γ.ix_inv (Γ.ix n) = n
+  := by {
+    revert n;
+    induction Γ with
+    | nil => intro n H; rfl
+    | cons H Γ I =>
+      intro n;
+      cases n with
+      | zero => 
+        intro Hn;
+        cases H with
+        | true => rfl
+        | false => simp [List.get?] at Hn
+      | succ n =>
+        intro Hn;
+        cases H <;> simp [ix, ix_inv, I Hn] 
+  }
